Fixed suggestions

src/specs/PermutationQuotientContribution.ec
@@ -6,48 +6,46 @@ require import UInt256.
 require import Verifier.
 require import YulPrimops.
 require import Utils.
-require        VerifierConsts.
-require        VerifierVars.
-require        VerifierMem.
-
-import VerifierConsts VerifierVars.
+require import VerifierConsts.
+require import VerifierVars.
+require import VerifierMem.
 
 module PermutationQuotientContribution = {
   proc low(): uint256 = {
-    var usr_res, tmp270, tmp271, usr_gamma, usr_beta, usr_factorMultiplier, tmp274, tmp275, tmp276, tmp277, tmp278, tmp279, tmp280, _22, usr_l0AtZ, tmp282, _26;
+    var _res, tmp270, tmp271, _gamma, _beta, _factorMultiplier, tmp274, tmp275, tmp276, tmp277, tmp278, tmp279, tmp280, _22, usr_l0AtZ, tmp282, _26;
     tmp270 <@ Primops.mload(STATE_POWER_OF_ALPHA_4_SLOT);
     tmp271 <@ Primops.mload(PROOF_COPY_PERMUTATION_GRAND_PRODUCT_OPENING_AT_Z_OMEGA_SLOT);
-    usr_res <- (PurePrimops.mulmod tmp271 tmp270 (W256.of_int Constants.R));
-    usr_gamma <@ Primops.mload(STATE_GAMMA_SLOT);
-    usr_beta <@ Primops.mload(STATE_BETA_SLOT);
+    _res <- (PurePrimops.mulmod tmp271 tmp270 (W256.of_int Constants.R));
+    _gamma <@ Primops.mload(STATE_GAMMA_SLOT);
+    _beta <@ Primops.mload(STATE_BETA_SLOT);
     tmp274 <@ Primops.mload(PROOF_COPY_PERMUTATION_POLYS_0_OPENING_AT_Z_SLOT);
-    usr_factorMultiplier <- (PurePrimops.mulmod tmp274 usr_beta (W256.of_int Constants.R));
-    usr_factorMultiplier <- (PurePrimops.addmod usr_factorMultiplier usr_gamma (W256.of_int Constants.R));
+    _factorMultiplier <- (PurePrimops.mulmod tmp274 _beta (W256.of_int Constants.R));
+    _factorMultiplier <- (PurePrimops.addmod _factorMultiplier _gamma (W256.of_int Constants.R));
     tmp275 <@ Primops.mload(PROOF_STATE_POLYS_0_OPENING_AT_Z_SLOT);
-    usr_factorMultiplier <- (PurePrimops.addmod usr_factorMultiplier tmp275 (W256.of_int Constants.R));
-    usr_res <- (PurePrimops.mulmod usr_res usr_factorMultiplier (W256.of_int Constants.R));
+    _factorMultiplier <- (PurePrimops.addmod _factorMultiplier tmp275 (W256.of_int Constants.R));
+    _res <- (PurePrimops.mulmod _res _factorMultiplier (W256.of_int Constants.R));
     tmp276 <@ Primops.mload(PROOF_COPY_PERMUTATION_POLYS_1_OPENING_AT_Z_SLOT);
-    usr_factorMultiplier <- (PurePrimops.mulmod tmp276 usr_beta (W256.of_int Constants.R));
-    usr_factorMultiplier <- (PurePrimops.addmod usr_factorMultiplier usr_gamma (W256.of_int Constants.R));
+    _factorMultiplier <- (PurePrimops.mulmod tmp276 _beta (W256.of_int Constants.R));
+    _factorMultiplier <- (PurePrimops.addmod _factorMultiplier _gamma (W256.of_int Constants.R));
     tmp277 <@ Primops.mload(PROOF_STATE_POLYS_1_OPENING_AT_Z_SLOT);
-    usr_factorMultiplier <- (PurePrimops.addmod usr_factorMultiplier tmp277 (W256.of_int Constants.R));
-    usr_res <- (PurePrimops.mulmod usr_res usr_factorMultiplier (W256.of_int Constants.R));
+    _factorMultiplier <- (PurePrimops.addmod _factorMultiplier tmp277 (W256.of_int Constants.R));
+    _res <- (PurePrimops.mulmod _res _factorMultiplier (W256.of_int Constants.R));
     tmp278 <@ Primops.mload(PROOF_COPY_PERMUTATION_POLYS_2_OPENING_AT_Z_SLOT);
-    usr_factorMultiplier <- (PurePrimops.mulmod tmp278 usr_beta (W256.of_int Constants.R));
-    usr_factorMultiplier <- (PurePrimops.addmod usr_factorMultiplier usr_gamma (W256.of_int Constants.R));
+    _factorMultiplier <- (PurePrimops.mulmod tmp278 _beta (W256.of_int Constants.R));
+    _factorMultiplier <- (PurePrimops.addmod _factorMultiplier _gamma (W256.of_int Constants.R));
     tmp279 <@ Primops.mload(PROOF_STATE_POLYS_2_OPENING_AT_Z_SLOT);
-    usr_factorMultiplier <- (PurePrimops.addmod usr_factorMultiplier tmp279 (W256.of_int Constants.R));
-    usr_res <- (PurePrimops.mulmod usr_res usr_factorMultiplier (W256.of_int Constants.R));
+    _factorMultiplier <- (PurePrimops.addmod _factorMultiplier tmp279 (W256.of_int Constants.R));
+    _res <- (PurePrimops.mulmod _res _factorMultiplier (W256.of_int Constants.R));
     tmp280 <@ Primops.mload(PROOF_STATE_POLYS_3_OPENING_AT_Z_SLOT);
-    _22 <- (PurePrimops.addmod tmp280 usr_gamma (W256.of_int Constants.R));
-    usr_res <- (PurePrimops.mulmod usr_res _22 (W256.of_int Constants.R));
-    usr_res <- ((W256.of_int Constants.R) - usr_res);
+    _22 <- (PurePrimops.addmod tmp280 _gamma (W256.of_int Constants.R));
+    _res <- (PurePrimops.mulmod _res _22 (W256.of_int Constants.R));
+    _res <- ((W256.of_int Constants.R) - _res);
     usr_l0AtZ <@ Primops.mload(STATE_L_0_AT_Z_SLOT);
     tmp282 <@ Primops.mload(STATE_POWER_OF_ALPHA_5_SLOT);
     usr_l0AtZ <- (PurePrimops.mulmod usr_l0AtZ tmp282 (W256.of_int Constants.R));
     _26 <- ((W256.of_int Constants.R) - usr_l0AtZ);
-    usr_res <- (PurePrimops.addmod usr_res _26 (W256.of_int Constants.R));
-    return usr_res;
+    _res <- (PurePrimops.addmod _res _26 (W256.of_int Constants.R));
+    return _res;
   }
 
   proc mid() : int = {
@@ -73,17 +71,17 @@ lemma permutationQuotientContribution_extracted_equiv_low:
     ].
 proof. proc.
   inline *; wp; skip; progress; by smt ().
-qed. 
+qed.
 
 section.
 
 local module TMP = {
   proc low1(): uint256 = {
-    var usr_res, _alpha4, _zperm_zOmega, usr_gamma, usr_beta, usr_factorMultiplier, _sigma0_z, _a_z, _sigma1_z, _b_z, _sigma2_z, _c_z, _sigma3_z, _22, usr_l0AtZ, _alpha5, _26;
+    var _res, _alpha4, _zperm_zOmega, _gamma, _beta, _factorMultiplier, _sigma0_z, _a_z, _sigma1_z, _b_z, _sigma2_z, _c_z, _sigma3_z, _22, usr_l0AtZ, _alpha5, _26;
     _alpha4 <@ Primops.mload(STATE_POWER_OF_ALPHA_4_SLOT);
     _zperm_zOmega <@ Primops.mload(PROOF_COPY_PERMUTATION_GRAND_PRODUCT_OPENING_AT_Z_OMEGA_SLOT);
-    usr_gamma <@ Primops.mload(STATE_GAMMA_SLOT);
-    usr_beta <@ Primops.mload(STATE_BETA_SLOT);
+    _gamma <@ Primops.mload(STATE_GAMMA_SLOT);
+    _beta <@ Primops.mload(STATE_BETA_SLOT);
     _sigma0_z <@ Primops.mload(PROOF_COPY_PERMUTATION_POLYS_0_OPENING_AT_Z_SLOT);
     _a_z <@ Primops.mload(PROOF_STATE_POLYS_0_OPENING_AT_Z_SLOT);
     _sigma1_z <@ Primops.mload(PROOF_COPY_PERMUTATION_POLYS_1_OPENING_AT_Z_SLOT);
@@ -94,36 +92,36 @@ local module TMP = {
     usr_l0AtZ <@ Primops.mload(STATE_L_0_AT_Z_SLOT);
     _alpha5 <@ Primops.mload(STATE_POWER_OF_ALPHA_5_SLOT);
     
-    usr_res <- (PurePrimops.mulmod _zperm_zOmega _alpha4 (W256.of_int Constants.R));
-    usr_factorMultiplier <- (PurePrimops.mulmod _sigma0_z usr_beta (W256.of_int Constants.R));
-    usr_factorMultiplier <- (PurePrimops.addmod usr_factorMultiplier usr_gamma (W256.of_int Constants.R));
-    usr_factorMultiplier <- (PurePrimops.addmod usr_factorMultiplier _a_z (W256.of_int Constants.R));
-    usr_res <- (PurePrimops.mulmod usr_res usr_factorMultiplier (W256.of_int Constants.R));
-    usr_factorMultiplier <- (PurePrimops.mulmod _sigma1_z usr_beta (W256.of_int Constants.R));
-    usr_factorMultiplier <- (PurePrimops.addmod usr_factorMultiplier usr_gamma (W256.of_int Constants.R));
-    usr_factorMultiplier <- (PurePrimops.addmod usr_factorMultiplier _b_z (W256.of_int Constants.R));
-    usr_res <- (PurePrimops.mulmod usr_res usr_factorMultiplier (W256.of_int Constants.R));
-    usr_factorMultiplier <- (PurePrimops.mulmod _sigma2_z usr_beta (W256.of_int Constants.R));
-    usr_factorMultiplier <- (PurePrimops.addmod usr_factorMultiplier usr_gamma (W256.of_int Constants.R));
-    usr_factorMultiplier <- (PurePrimops.addmod usr_factorMultiplier _c_z (W256.of_int Constants.R));
-    usr_res <- (PurePrimops.mulmod usr_res usr_factorMultiplier (W256.of_int Constants.R));
-    _22 <- (PurePrimops.addmod _sigma3_z usr_gamma (W256.of_int Constants.R));
-    usr_res <- (PurePrimops.mulmod usr_res _22 (W256.of_int Constants.R));
-    usr_res <- ((W256.of_int Constants.R) - usr_res);
+    _res <- (PurePrimops.mulmod _zperm_zOmega _alpha4 (W256.of_int Constants.R));
+    _factorMultiplier <- (PurePrimops.mulmod _sigma0_z _beta (W256.of_int Constants.R));
+    _factorMultiplier <- (PurePrimops.addmod _factorMultiplier _gamma (W256.of_int Constants.R));
+    _factorMultiplier <- (PurePrimops.addmod _factorMultiplier _a_z (W256.of_int Constants.R));
+    _res <- (PurePrimops.mulmod _res _factorMultiplier (W256.of_int Constants.R));
+    _factorMultiplier <- (PurePrimops.mulmod _sigma1_z _beta (W256.of_int Constants.R));
+    _factorMultiplier <- (PurePrimops.addmod _factorMultiplier _gamma (W256.of_int Constants.R));
+    _factorMultiplier <- (PurePrimops.addmod _factorMultiplier _b_z (W256.of_int Constants.R));
+    _res <- (PurePrimops.mulmod _res _factorMultiplier (W256.of_int Constants.R));
+    _factorMultiplier <- (PurePrimops.mulmod _sigma2_z _beta (W256.of_int Constants.R));
+    _factorMultiplier <- (PurePrimops.addmod _factorMultiplier _gamma (W256.of_int Constants.R));
+    _factorMultiplier <- (PurePrimops.addmod _factorMultiplier _c_z (W256.of_int Constants.R));
+    _res <- (PurePrimops.mulmod _res _factorMultiplier (W256.of_int Constants.R));
+    _22 <- (PurePrimops.addmod _sigma3_z _gamma (W256.of_int Constants.R));
+    _res <- (PurePrimops.mulmod _res _22 (W256.of_int Constants.R));
+    _res <- ((W256.of_int Constants.R) - _res);
     usr_l0AtZ <- (PurePrimops.mulmod usr_l0AtZ _alpha5 (W256.of_int Constants.R));
     _26 <- ((W256.of_int Constants.R) - usr_l0AtZ);
-    usr_res <- (PurePrimops.addmod usr_res _26 (W256.of_int Constants.R));
-    return usr_res;
+    _res <- (PurePrimops.addmod _res _26 (W256.of_int Constants.R));
+    return _res;
   }
 
   proc low2(): uint256 = {
-    var usr_res, _alpha4, _zperm_zOmega, usr_gamma, usr_beta, usr_factorMultiplier, _sigma0_z, _a_z, _sigma1_z, _b_z, _sigma2_z, _c_z, _sigma3_z, usr_l0AtZ, _alpha5, _26;
+    var _res, _alpha4, _zperm_zOmega, _gamma, _beta, _factorMultiplier, _sigma0_z, _a_z, _sigma1_z, _b_z, _sigma2_z, _c_z, _sigma3_z, usr_l0AtZ, _alpha5, _26;
     var s0BGa, s1BGb, s2BGc, s3G;
     
     _alpha4 <@ Primops.mload(STATE_POWER_OF_ALPHA_4_SLOT);
     _zperm_zOmega <@ Primops.mload(PROOF_COPY_PERMUTATION_GRAND_PRODUCT_OPENING_AT_Z_OMEGA_SLOT);
-    usr_gamma <@ Primops.mload(STATE_GAMMA_SLOT);
-    usr_beta <@ Primops.mload(STATE_BETA_SLOT);
+    _gamma <@ Primops.mload(STATE_GAMMA_SLOT);
+    _beta <@ Primops.mload(STATE_BETA_SLOT);
     _sigma0_z <@ Primops.mload(PROOF_COPY_PERMUTATION_POLYS_0_OPENING_AT_Z_SLOT);
     _a_z <@ Primops.mload(PROOF_STATE_POLYS_0_OPENING_AT_Z_SLOT);
     _sigma1_z <@ Primops.mload(PROOF_COPY_PERMUTATION_POLYS_1_OPENING_AT_Z_SLOT);
@@ -134,48 +132,48 @@ local module TMP = {
     usr_l0AtZ <@ Primops.mload(STATE_L_0_AT_Z_SLOT);
     _alpha5 <@ Primops.mload(STATE_POWER_OF_ALPHA_5_SLOT);
     
-    usr_res <- (PurePrimops.mulmod _zperm_zOmega _alpha4 (W256.of_int Constants.R));
+    _res <- (PurePrimops.mulmod _zperm_zOmega _alpha4 (W256.of_int Constants.R));
     
-    s0BGa <- (PurePrimops.mulmod _sigma0_z usr_beta (W256.of_int Constants.R));
-    s0BGa <- (PurePrimops.addmod s0BGa usr_gamma (W256.of_int Constants.R));
+    s0BGa <- (PurePrimops.mulmod _sigma0_z _beta (W256.of_int Constants.R));
+    s0BGa <- (PurePrimops.addmod s0BGa _gamma (W256.of_int Constants.R));
     s0BGa <- (PurePrimops.addmod s0BGa _a_z (W256.of_int Constants.R));
 
-    usr_factorMultiplier <- s0BGa;
-    usr_res <- (PurePrimops.mulmod usr_res usr_factorMultiplier (W256.of_int Constants.R));
+    _factorMultiplier <- s0BGa;
+    _res <- (PurePrimops.mulmod _res _factorMultiplier (W256.of_int Constants.R));
     
-    s1BGb <- (PurePrimops.mulmod _sigma1_z usr_beta (W256.of_int Constants.R));
-    s1BGb <- (PurePrimops.addmod s1BGb usr_gamma (W256.of_int Constants.R));
+    s1BGb <- (PurePrimops.mulmod _sigma1_z _beta (W256.of_int Constants.R));
+    s1BGb <- (PurePrimops.addmod s1BGb _gamma (W256.of_int Constants.R));
     s1BGb <- (PurePrimops.addmod s1BGb _b_z (W256.of_int Constants.R));
 
-    usr_factorMultiplier <- s1BGb;
-    usr_res <- (PurePrimops.mulmod usr_res usr_factorMultiplier (W256.of_int Constants.R));
+    _factorMultiplier <- s1BGb;
+    _res <- (PurePrimops.mulmod _res _factorMultiplier (W256.of_int Constants.R));
 
-    s2BGc <- (PurePrimops.mulmod _sigma2_z usr_beta (W256.of_int Constants.R));
-    s2BGc <- (PurePrimops.addmod s2BGc usr_gamma (W256.of_int Constants.R));
+    s2BGc <- (PurePrimops.mulmod _sigma2_z _beta (W256.of_int Constants.R));
+    s2BGc <- (PurePrimops.addmod s2BGc _gamma (W256.of_int Constants.R));
     s2BGc <- (PurePrimops.addmod s2BGc _c_z (W256.of_int Constants.R));
 
-    usr_factorMultiplier <- s2BGc;
-    usr_res <- (PurePrimops.mulmod usr_res usr_factorMultiplier (W256.of_int Constants.R));
+    _factorMultiplier <- s2BGc;
+    _res <- (PurePrimops.mulmod _res _factorMultiplier (W256.of_int Constants.R));
 
-    s3G   <- (PurePrimops.addmod _sigma3_z usr_gamma (W256.of_int Constants.R));
-    usr_res <- (PurePrimops.mulmod usr_res s3G (W256.of_int Constants.R));
+    s3G   <- (PurePrimops.addmod _sigma3_z _gamma (W256.of_int Constants.R));
+    _res <- (PurePrimops.mulmod _res s3G (W256.of_int Constants.R));
     
-    usr_res <- ((W256.of_int Constants.R) - usr_res);
+    _res <- ((W256.of_int Constants.R) - _res);
     usr_l0AtZ <- (PurePrimops.mulmod usr_l0AtZ _alpha5 (W256.of_int Constants.R));
     _26 <- ((W256.of_int Constants.R) - usr_l0AtZ);
-    usr_res <- (PurePrimops.addmod usr_res _26 (W256.of_int Constants.R));
-    return usr_res;
+    _res <- (PurePrimops.addmod _res _26 (W256.of_int Constants.R));
+    return _res;
   }
 
   proc low3(): uint256 = {
-    var usr_res1, usr_res2, _alpha4, _zperm_zOmega, usr_gamma, usr_beta, _sigma0_z, _a_z, _sigma1_z, _b_z, _sigma2_z, _c_z, _sigma3_z, usr_l0AtZ, _alpha5;
+    var _res1, _res2, _alpha4, _zperm_zOmega, _gamma, _beta, _sigma0_z, _a_z, _sigma1_z, _b_z, _sigma2_z, _c_z, _sigma3_z, usr_l0AtZ, _alpha5;
     var s0BGa, s1BGb, s2BGc, s3G;
     var inv1, inv2;
     
     _alpha4 <@ Primops.mload(STATE_POWER_OF_ALPHA_4_SLOT);
     _zperm_zOmega <@ Primops.mload(PROOF_COPY_PERMUTATION_GRAND_PRODUCT_OPENING_AT_Z_OMEGA_SLOT);
-    usr_gamma <@ Primops.mload(STATE_GAMMA_SLOT);
-    usr_beta <@ Primops.mload(STATE_BETA_SLOT);
+    _gamma <@ Primops.mload(STATE_GAMMA_SLOT);
+    _beta <@ Primops.mload(STATE_BETA_SLOT);
     _sigma0_z <@ Primops.mload(PROOF_COPY_PERMUTATION_POLYS_0_OPENING_AT_Z_SLOT);
     _a_z <@ Primops.mload(PROOF_STATE_POLYS_0_OPENING_AT_Z_SLOT);
     _sigma1_z <@ Primops.mload(PROOF_COPY_PERMUTATION_POLYS_1_OPENING_AT_Z_SLOT);
@@ -186,45 +184,45 @@ local module TMP = {
     usr_l0AtZ <@ Primops.mload(STATE_L_0_AT_Z_SLOT);
     _alpha5 <@ Primops.mload(STATE_POWER_OF_ALPHA_5_SLOT);
     
-    usr_res1 <- (PurePrimops.mulmod _zperm_zOmega _alpha4 (W256.of_int Constants.R));
+    _res1 <- (PurePrimops.mulmod _zperm_zOmega _alpha4 (W256.of_int Constants.R));
     
-    s0BGa <- (PurePrimops.mulmod _sigma0_z usr_beta (W256.of_int Constants.R));
-    s0BGa <- (PurePrimops.addmod s0BGa usr_gamma (W256.of_int Constants.R));
+    s0BGa <- (PurePrimops.mulmod _sigma0_z _beta (W256.of_int Constants.R));
+    s0BGa <- (PurePrimops.addmod s0BGa _gamma (W256.of_int Constants.R));
     s0BGa <- (PurePrimops.addmod s0BGa _a_z (W256.of_int Constants.R));
 
-    usr_res1 <- (PurePrimops.mulmod usr_res1 s0BGa (W256.of_int Constants.R));
+    _res1 <- (PurePrimops.mulmod _res1 s0BGa (W256.of_int Constants.R));
     
-    s1BGb <- (PurePrimops.mulmod _sigma1_z usr_beta (W256.of_int Constants.R));
-    s1BGb <- (PurePrimops.addmod s1BGb usr_gamma (W256.of_int Constants.R));
+    s1BGb <- (PurePrimops.mulmod _sigma1_z _beta (W256.of_int Constants.R));
+    s1BGb <- (PurePrimops.addmod s1BGb _gamma (W256.of_int Constants.R));
     s1BGb <- (PurePrimops.addmod s1BGb _b_z (W256.of_int Constants.R));
 
-    usr_res1 <- (PurePrimops.mulmod usr_res1 s1BGb (W256.of_int Constants.R));
+    _res1 <- (PurePrimops.mulmod _res1 s1BGb (W256.of_int Constants.R));
 
-    s2BGc <- (PurePrimops.mulmod _sigma2_z usr_beta (W256.of_int Constants.R));
-    s2BGc <- (PurePrimops.addmod s2BGc usr_gamma (W256.of_int Constants.R));
+    s2BGc <- (PurePrimops.mulmod _sigma2_z _beta (W256.of_int Constants.R));
+    s2BGc <- (PurePrimops.addmod s2BGc _gamma (W256.of_int Constants.R));
     s2BGc <- (PurePrimops.addmod s2BGc _c_z (W256.of_int Constants.R));
 
-    usr_res1 <- (PurePrimops.mulmod usr_res1 s2BGc (W256.of_int Constants.R));
+    _res1 <- (PurePrimops.mulmod _res1 s2BGc (W256.of_int Constants.R));
 
-    s3G   <- (PurePrimops.addmod _sigma3_z usr_gamma (W256.of_int Constants.R));
-    usr_res1 <- (PurePrimops.mulmod usr_res1 s3G (W256.of_int Constants.R));
-    inv1 <- ((W256.of_int Constants.R) - usr_res1);
+    s3G   <- (PurePrimops.addmod _sigma3_z _gamma (W256.of_int Constants.R));
+    _res1 <- (PurePrimops.mulmod _res1 s3G (W256.of_int Constants.R));
+    inv1 <- ((W256.of_int Constants.R) - _res1);
     
-    usr_res2 <- (PurePrimops.mulmod usr_l0AtZ _alpha5 (W256.of_int Constants.R));
-    inv2 <- ((W256.of_int Constants.R) - usr_res2);
+    _res2 <- (PurePrimops.mulmod usr_l0AtZ _alpha5 (W256.of_int Constants.R));
+    inv2 <- ((W256.of_int Constants.R) - _res2);
 
     return (PurePrimops.addmod inv1 inv2 (W256.of_int Constants.R));
   }
 
   proc low4(): uint256 = {
-    var usr_res1, usr_res2, _alpha4, _zperm_zOmega, usr_gamma, usr_beta, _sigma0_z, _a_z, _sigma1_z, _b_z, _sigma2_z, _c_z, _sigma3_z, usr_l0AtZ, _alpha5;
+    var _res1, _res2, _alpha4, _zperm_zOmega, _gamma, _beta, _sigma0_z, _a_z, _sigma1_z, _b_z, _sigma2_z, _c_z, _sigma3_z, usr_l0AtZ, _alpha5;
     var s0BGa, s1BGb, s2BGc, s3G;
     var inv1, inv2;
     
     _alpha4 <@ Primops.mload(STATE_POWER_OF_ALPHA_4_SLOT);
     _zperm_zOmega <@ Primops.mload(PROOF_COPY_PERMUTATION_GRAND_PRODUCT_OPENING_AT_Z_OMEGA_SLOT);
-    usr_gamma <@ Primops.mload(STATE_GAMMA_SLOT);
-    usr_beta <@ Primops.mload(STATE_BETA_SLOT);
+    _gamma <@ Primops.mload(STATE_GAMMA_SLOT);
+    _beta <@ Primops.mload(STATE_BETA_SLOT);
     _sigma0_z <@ Primops.mload(PROOF_COPY_PERMUTATION_POLYS_0_OPENING_AT_Z_SLOT);
     _a_z <@ Primops.mload(PROOF_STATE_POLYS_0_OPENING_AT_Z_SLOT);
     _sigma1_z <@ Primops.mload(PROOF_COPY_PERMUTATION_POLYS_1_OPENING_AT_Z_SLOT);
@@ -235,29 +233,29 @@ local module TMP = {
     usr_l0AtZ <@ Primops.mload(STATE_L_0_AT_Z_SLOT);
     _alpha5 <@ Primops.mload(STATE_POWER_OF_ALPHA_5_SLOT);
     
-    s0BGa <- (PurePrimops.mulmod _sigma0_z usr_beta (W256.of_int Constants.R));
-    s0BGa <- (PurePrimops.addmod s0BGa usr_gamma (W256.of_int Constants.R));
+    s0BGa <- (PurePrimops.mulmod _sigma0_z _beta (W256.of_int Constants.R));
+    s0BGa <- (PurePrimops.addmod s0BGa _gamma (W256.of_int Constants.R));
     s0BGa <- (PurePrimops.addmod s0BGa _a_z (W256.of_int Constants.R));
     
-    s1BGb <- (PurePrimops.mulmod _sigma1_z usr_beta (W256.of_int Constants.R));
-    s1BGb <- (PurePrimops.addmod s1BGb usr_gamma (W256.of_int Constants.R));
+    s1BGb <- (PurePrimops.mulmod _sigma1_z _beta (W256.of_int Constants.R));
+    s1BGb <- (PurePrimops.addmod s1BGb _gamma (W256.of_int Constants.R));
     s1BGb <- (PurePrimops.addmod s1BGb _b_z (W256.of_int Constants.R));
 
-    s2BGc <- (PurePrimops.mulmod _sigma2_z usr_beta (W256.of_int Constants.R));
-    s2BGc <- (PurePrimops.addmod s2BGc usr_gamma (W256.of_int Constants.R));
+    s2BGc <- (PurePrimops.mulmod _sigma2_z _beta (W256.of_int Constants.R));
+    s2BGc <- (PurePrimops.addmod s2BGc _gamma (W256.of_int Constants.R));
     s2BGc <- (PurePrimops.addmod s2BGc _c_z (W256.of_int Constants.R));
 
-    s3G   <- (PurePrimops.addmod _sigma3_z usr_gamma (W256.of_int Constants.R));
+    s3G   <- (PurePrimops.addmod _sigma3_z _gamma (W256.of_int Constants.R));
 
-    usr_res1 <- (PurePrimops.mulmod _zperm_zOmega _alpha4 (W256.of_int Constants.R));
-    usr_res1 <- (PurePrimops.mulmod usr_res1 s0BGa (W256.of_int Constants.R));
-    usr_res1 <- (PurePrimops.mulmod usr_res1 s1BGb (W256.of_int Constants.R));
-    usr_res1 <- (PurePrimops.mulmod usr_res1 s2BGc (W256.of_int Constants.R));
-    usr_res1 <- (PurePrimops.mulmod usr_res1 s3G (W256.of_int Constants.R));
-    inv1 <- ((W256.of_int Constants.R) - usr_res1);
+    _res1 <- (PurePrimops.mulmod _zperm_zOmega _alpha4 (W256.of_int Constants.R));
+    _res1 <- (PurePrimops.mulmod _res1 s0BGa (W256.of_int Constants.R));
+    _res1 <- (PurePrimops.mulmod _res1 s1BGb (W256.of_int Constants.R));
+    _res1 <- (PurePrimops.mulmod _res1 s2BGc (W256.of_int Constants.R));
+    _res1 <- (PurePrimops.mulmod _res1 s3G (W256.of_int Constants.R));
+    inv1 <- ((W256.of_int Constants.R) - _res1);
     
-    usr_res2 <- (PurePrimops.mulmod usr_l0AtZ _alpha5 (W256.of_int Constants.R));
-    inv2 <- ((W256.of_int Constants.R) - usr_res2);
+    _res2 <- (PurePrimops.mulmod usr_l0AtZ _alpha5 (W256.of_int Constants.R));
+    inv2 <- ((W256.of_int Constants.R) - _res2);
 
     return (PurePrimops.addmod inv1 inv2 (W256.of_int Constants.R));
   }
@@ -266,82 +264,154 @@ local module TMP = {
 
 local lemma low_equiv_low1 :
 equiv [PermutationQuotientContribution.low ~ TMP.low1 :
-      ={arg, Primops.memory} ==> ={res, Primops.memory}].
+      ={arg, Primops.memory} /\
+      !Primops.reverted{1} /\ !Primops.reverted{2}
+      ==>
+      ={res, Primops.memory} /\
+      !Primops.reverted{1} /\ !Primops.reverted{2}
+    ].
 proof. proc.
   inline *; wp; skip; progress; smt ().
 qed.
 
 local lemma low1_equiv_low2 :
-     equiv [TMP.low1 ~ TMP.low2 : ={arg, glob TMP} ==> ={res, glob TMP}].
+equiv [TMP.low1 ~ TMP.low2 :
+      ={arg, glob TMP} /\
+      !Primops.reverted{1} /\ !Primops.reverted{2}
+      ==>
+      ={res, glob TMP} /\
+      !Primops.reverted{1} /\ !Primops.reverted{2}
+    ].
 proof. proc.
   inline *; wp; skip; progress; smt ().
 qed.
 
 local lemma low2_equiv_low3 :
-     equiv [TMP.low2 ~ TMP.low3 : ={arg, glob TMP} ==> ={res, glob TMP}].
+equiv [TMP.low2 ~ TMP.low3 :
+      ={arg, glob TMP} /\
+      !Primops.reverted{1} /\ !Primops.reverted{2}
+      ==>
+      ={res, glob TMP} /\
+      !Primops.reverted{1} /\ !Primops.reverted{2}
+    ].
 proof. proc.
   inline *; wp; skip; progress; smt ().
 qed.
 
 local lemma low3_equiv_low4 :
-     equiv [TMP.low3 ~ TMP.low4 : ={arg, glob TMP} ==> ={res, glob TMP}].
+equiv [TMP.low3 ~ TMP.low4 :
+      ={arg, glob TMP} /\
+      !Primops.reverted{1} /\ !Primops.reverted{2}
+      ==>
+      ={res, glob TMP} /\
+      !Primops.reverted{1} /\ !Primops.reverted{2}
+    ].
 proof. proc.
   inline *; wp; skip; progress; smt ().
 qed.
 
 local lemma low_equiv_low4 :
 equiv [PermutationQuotientContribution.low ~ TMP.low4 :
-      ={arg, Primops.memory} ==> ={res, Primops.memory}].
+      ={arg, Primops.memory} /\
+      !Primops.reverted{1} /\ !Primops.reverted{2}
+      ==>
+      ={res, Primops.memory} /\
+      !Primops.reverted{1} /\ !Primops.reverted{2}
+    ].
 proof.
-transitivity TMP.low1 (={arg, glob PermutationQuotientContribution} ==> ={res, glob PermutationQuotientContribution}) (={arg, Primops.memory} ==> ={res, Primops.memory}); progress.
-exists Primops.memory{2}. progress. apply low_equiv_low1.
-transitivity TMP.low2 (={arg, glob TMP} ==> ={res, glob TMP}) (={arg, glob TMP} ==> ={res, glob TMP}); progress.
-exists Primops.memory{2}. progress. apply low1_equiv_low2.
-transitivity TMP.low3 (={arg, glob TMP} ==> ={res, glob TMP}) (={arg, glob TMP} ==> ={res, glob TMP}); progress.
-exists Primops.memory{2}. progress. apply low2_equiv_low3.
+transitivity TMP.low1
+(={arg, Primops.memory} /\
+      !Primops.reverted{1} /\ !Primops.reverted{2}
+      ==>
+      ={res, Primops.memory} /\
+      !Primops.reverted{1} /\ !Primops.reverted{2})
+
+(={arg, glob TMP} /\
+      !Primops.reverted{1} /\ !Primops.reverted{2}
+      ==>
+      ={res, glob TMP} /\
+      !Primops.reverted{1} /\ !Primops.reverted{2}); progress.
+exists Primops.memory{2} Primops.reverted{1}; progress. apply low_equiv_low1.
+transitivity TMP.low2 (={arg, glob TMP} /\
+      !Primops.reverted{1} /\ !Primops.reverted{2}
+      ==>
+      ={res, glob TMP} /\
+      !Primops.reverted{1} /\ !Primops.reverted{2}) (={arg, glob TMP} /\
+      !Primops.reverted{1} /\ !Primops.reverted{2}
+      ==>
+      ={res, glob TMP} /\
+      !Primops.reverted{1} /\ !Primops.reverted{2}); progress.
+exists Primops.memory{2} Primops.reverted{1}. progress. apply low1_equiv_low2.
+transitivity TMP.low3 (={arg, glob TMP} /\
+      !Primops.reverted{1} /\ !Primops.reverted{2}
+      ==>
+      ={res, glob TMP} /\
+      !Primops.reverted{1} /\ !Primops.reverted{2}) (={arg, glob TMP} /\
+      !Primops.reverted{1} /\ !Primops.reverted{2}
+      ==>
+      ={res, glob TMP} /\
+      !Primops.reverted{1} /\ !Primops.reverted{2}); progress.
+exists Primops.memory{2} Primops.reverted{1}. progress. apply low2_equiv_low3.
 apply low3_equiv_low4.
 qed.
 
 import MemoryMap VerifierMem.
 declare op m : mem.
 
-pred permutationQuotientContribution_pre_mem = 
-  alpha4_mem m /\ alpha5_mem m /\ beta_mem m /\ gamma_mem m /\
-  sigma0_z_mem m /\ sigma1_z_mem m /\ sigma2_z_mem m /\ sigma3_z_mem m /\
-  a_z_mem m /\ b_z_mem m /\ c_z_mem m /\  
-  zperm_zOmega_mem m /\ l0_z_mem m.
+pred permutationQuotientContribution_memory_vars = 
+  alpha4_mem m /\
+  alpha5_mem m /\
+  beta_mem m /\
+  gamma_mem m /\
+  sigma0_z_mem m /\
+  sigma1_z_mem m /\
+  sigma2_z_mem m /\
+  sigma3_z_mem m /\
+  a_z_mem m /\
+  b_z_mem m /\
+  c_z_mem m /\  
+  zperm_zOmega_mem m /\
+  l0_z_mem m.
 
 lemma low_equiv_mid :
 equiv [PermutationQuotientContribution.low ~ PermutationQuotientContribution.mid :
-   ={arg, glob PermutationQuotientContribution} /\
+   ={arg} /\
    Primops.memory{1} = m /\
-   !Primops.reverted{1} /\
-   !Primops.reverted{2} /\
-   permutationQuotientContribution_pre_mem
+   !Primops.reverted{1} /\ !Primops.reverted{2} /\
+   permutationQuotientContribution_memory_vars
    ==>
-   W256.to_uint res{1} = res{2}
+   !Primops.reverted{1} /\ !Primops.reverted{2} /\
+   Primops.memory{1} = m /\
+   res{2} = W256.to_uint res{1}
  ].
 proof. 
-
 transitivity
   TMP.low4
-  (={arg, glob PermutationQuotientContribution} ==> ={res, glob PermutationQuotientContribution})
-  (={arg, glob PermutationQuotientContribution} /\
+  ( ={arg, Primops.memory} /\
+      !Primops.reverted{1} /\ !Primops.reverted{2}
+      ==>
+      ={res, Primops.memory} /\
+      !Primops.reverted{1} /\ !Primops.reverted{2})
+  (={arg} /\
    Primops.memory{1} = m /\
-   !Primops.reverted{1} /\
-   !Primops.reverted{2} /\
-   permutationQuotientContribution_pre_mem
+   !Primops.reverted{1} /\ !Primops.reverted{2} /\
+   permutationQuotientContribution_memory_vars
    ==>
-   W256.to_uint res{1} = res{2}); progress.
-exists m Primops.reverted{1}; auto. apply low_equiv_low4.
-rewrite /permutationQuotientContribution_pre_mem. proc.
+   !Primops.reverted{1} /\ !Primops.reverted{2} /\
+   Primops.memory{1} = m /\
+   res{2} = W256.to_uint res{1}).
+progress; exists m Primops.reverted{1}; by auto.
+by progress.
+by apply low_equiv_low4.
+
+rewrite /permutationQuotientContribution_memory_vars; proc.
 
 seq 13 0 : (#pre /\
   W256.to_uint _alpha4{1} = Alpha4 /\
   W256.to_uint _alpha5{1} = Alpha5 /\
   W256.to_uint _zperm_zOmega{1} = Zperm_zOmega /\
-  W256.to_uint usr_gamma{1} = Gamma /\ 
-  W256.to_uint usr_beta{1} = Beta /\
+  W256.to_uint _gamma{1} = Gamma /\ 
+  W256.to_uint _beta{1} = Beta /\
   W256.to_uint _sigma0_z{1} = Sigma0_z /\
   W256.to_uint _sigma1_z{1} = Sigma1_z /\
   W256.to_uint _sigma2_z{1} = Sigma2_z /\
@@ -368,23 +438,23 @@ skip; by progress.
 seq 10 4 : (#pre /\ W256.to_uint s0BGa{1} = s0BGa{2} /\ W256.to_uint s1BGb{1} = s1BGb{2} /\ W256.to_uint s2BGc{1} = s2BGc{2} /\ W256.to_uint s2BGc{1} = s2BGc{2} /\ W256.to_uint s3G{1} = s3G{2}).
 wp; skip; rewrite /addmod /mulmod; progress; rewrite !W256.of_uintK; by smt().
 
-seq 5 0 : (#pre /\ W256.to_uint usr_res1{1} = (Alpha4 * Zperm_zOmega * s0BGa{2} * s1BGb{2} * s2BGc{2} * s3G{2}) %% Constants.R).
+seq 5 0 : (#pre /\ W256.to_uint _res1{1} = (Alpha4 * Zperm_zOmega * s0BGa{2} * s1BGb{2} * s2BGc{2} * s3G{2}) %% Constants.R).
 wp; skip; rewrite /addmod /mulmod; progress; rewrite !W256.of_uintK !R_mod_W256_R !mod_R_W256_mod_R; by smt().
 
 seq 1 1 : (#pre /\ W256.to_uint inv1{1} = inv1{2}).
 wp; skip; progress; rewrite -H27.
 have ->:
- (Constants.R - to_uint usr_res1{1}) = (Constants.R - to_uint usr_res1{1}) %% W256.modulus.
+ (Constants.R - to_uint _res1{1}) = (Constants.R - to_uint _res1{1}) %% W256.modulus.
  by smt().
 rewrite -W256.of_uintK; by smt(@W256).
 
-seq 1 0 : (#pre /\ W256.to_uint usr_res2{1} = (Alpha5 * L0_z) %% Constants.R).
+seq 1 0 : (#pre /\ W256.to_uint _res2{1} = (Alpha5 * L0_z) %% Constants.R).
 wp; skip; rewrite /addmod /mulmod; progress; rewrite !W256.of_uintK !R_mod_W256_R !mod_R_W256_mod_R; by smt().
 
 seq 1 1 : (#pre /\ W256.to_uint inv2{1} = inv2{2}).
 wp; skip; progress; rewrite -H28.
 have ->:
- (Constants.R - to_uint usr_res2{1}) = (Constants.R - to_uint usr_res2{1}) %% W256.modulus.
+ (Constants.R - to_uint _res2{1}) = (Constants.R - to_uint _res2{1}) %% W256.modulus.
  by smt().
 rewrite -W256.of_uintK; by smt(@W256).
 
@@ -395,4 +465,3 @@ qed.
 
 end section.
 
-print low_equiv_mid.
